{
 "cells": [
  {
   "cell_type": "markdown",
   "metadata": {},
   "source": [
    "# What we are doing here: the idea of adaptive correction\n",
    "We have a system which can be cheracterised with the following set of equatins:\n",
    "\n",
    "<a name=\"1\"></a>$ \\mathbf{x}_k = f(\\mathbf{x}_{k-1}, \\mathbf{u}_k, \\mathbf{w}_k) \\quad (1),$\n",
    "\n",
    "<a name=\"2\"></a>$\\mathbf{z}_k = h(\\mathbf{x}_k) + \\mathbf{v}_k \\quad (2),$\n",
    "    \n",
    "Where [(1)](#1) is state transition equation and [(2)](#2) is measurement equation, $\\mathbf w_k$ and $\\mathbf v_k$ are process and measurement noise respectively, $\\mathbf u_k$ is control vector.\n",
    "\n",
    "We use the Extended Kalman Filter (EKF) as our main estimation algorithm and the $H_\\infty$ filter as backup algorithm to deal with Kalman filter divergenсe.\n",
    "\n",
    "# The EKF algorithm\n",
    "## Prediction step\n",
    "<a name=\"3\"></a>$\\mathbf{x}_{k|k-1} = f(\\mathbf{x}_{k-1|k-1}, \\mathbf{u}_k, 0) \\quad (3),$\n",
    "\n",
    "<a name=\"4\"></a>$\\mathbf{P}_{k|k-1} =  {\\mathbf{F}_{k}} \\mathbf{P}_{k-1|k-1} {\\mathbf{F}_{k}^\\top} + {\\mathbf{B}_{k}} {\\mathbf{Q}_{k}} {\\mathbf{B}_{k}^\\top} \\quad (4),$\n",
    "\n",
    "<a name=\"5\"></a>$\\mathbf{y}_{k} = \\mathbf{z}_{k} - h(\\mathbf{x}_{k|k-1}) \\quad (5),$\n",
    "\n",
    "## Correction step\n",
    "The convenient form of correction step is:\n",
    "\n",
    "<a name=\"6\"></a>$\\mathbf{S}_{k} = {{\\mathbf{H}_{k}}}\\mathbf{P}_{k|k-1}{{\\mathbf{H}_{k}^\\top}} + \\mathbf{R}_{k} \\quad (6),$\n",
    "\n",
    "<a name=\"7\"></a>$\\mathbf{K}_{k} = \\mathbf{P}_{k|k-1}{{\\mathbf{H}_{k}^\\top}}\\mathbf{S}_{k}^{-1} \\quad (7),$\n",
    "\n",
    "<a name=\"8\"></a>$\\mathbf{x}_{k|k} = \\mathbf{x}_{k|k-1} + \\mathbf{K}_{k} \\mathbf{y}_{k} \\quad (8),$\n",
    "\n",
    "<a name=\"9\"></a>$\\mathbf{P}_{k|k} = \\left(\\mathbf{I} - \\mathbf{K}_k \\mathbf{H}_k\\right) \\mathbf{P}_{k|k-1} \\left(\\mathbf{I} - \\mathbf{K}_k \\mathbf{H}_k\\right)^\\top + \\mathbf{K}_k \\mathbf{R}_k \\mathbf{K}_k^\\top \\quad (9),$\n",
    "\n",
    "To compare the EKF with the $H_\\infty$ filter we need to rewrite the correction step in the following form:\n",
    "\n",
    "<a name=\"10\"></a>$\\mathbf{P}_{k|k} = (\\mathbf{P}_{k|k-1}^{-1} + \\mathbf{H}_{k}^{\\top} \\mathbf{R}_{k}^{-1} \\mathbf{H}_{k} )^{-1} \\quad (10),$\n",
    "\n",
    "<a name=\"11\"></a>$\\mathbf{K}_{k} = \\mathbf{P}_{k|k}{{\\mathbf{H}_{k}^\\top}}\\mathbf{R}_{k}^{-1} \\quad (11),$\n",
    "\n",
    "<a name=\"12\"></a>$\\mathbf{x}_{k|k} = \\mathbf{x}_{k|k-1} + \\mathbf{K}_{k}\\mathbf{y}_{k} \\quad (12),$\n",
    "\n",
    "## Where:\n",
    "$ \\mathbf{F}_{k} = \\left . \\frac{\\partial f}{\\partial \\mathbf{x} } \\right \\vert _{\\mathbf{x}_{k-1|k-1},\\mathbf{u}_{k}}, \\quad $ \n",
    "$ \\mathbf{B}_{k} = \\left . \\frac{\\partial f}{\\partial \\mathbf{v} } \\right \\vert _{\\mathbf{x}_{k-1|k-1},\\mathbf{u}_{k}}, \\quad $\n",
    "$ \\mathbf{H}_{k} = \\left . \\frac{\\partial h}{\\partial \\mathbf{x} } \\right \\vert _{\\mathbf{x}_{k|k-1}}, \\quad $\n",
    "$ \\mathbf{Q}_{k} \\ge 0 $ is the process noise covariance\n",
    "$ , \\quad \\mathbf{R}_{k} \\ge 0 $ is the measurement noise covariance\n",
    "\n",
    "\n",
    "# The $H_\\infty$ filter algorithm\n",
    "The $H_\\infty$ filter algorithm is given in [**[Banavar1992]**](#banavar) this algorithm can be written as follows:\n",
    "\n",
    "## Prediction step\n",
    "<a name=\"13\"></a>$\\mathbf{x}_{k|k-1} = f(\\mathbf{x}_{k-1|k-1}, \\mathbf{u}_k, 0) \\quad (13),$\n",
    "\n",
    "<a name=\"14\"></a>$\\mathbf{P}_{k|k-1} =  {\\mathbf{F}_{k}} \\mathbf{P}_{k-1|k-1} {\\mathbf{F}_{k}^\\top} + {\\mathbf{B}_{k}} {\\mathbf{Q}_{k}} {\\mathbf{B}_{k}^\\top} \\quad (14),$\n",
    "\n",
    "<a name=\"15\"></a>$\\mathbf{y}_{k} = \\mathbf{z}_{k} - h(\\mathbf{x}_{k|k-1}) \\quad (15),$\n",
    "\n",
    "## Correction step\n",
    "<a name=\"16\"></a>$\\mathbf{\\tilde{S}}_{k} =  {\\mathbf{L}_{b}^{\\top}} \\mathbf{\\bar{S}}_{k} {\\mathbf{L}_{k}} \\quad (16),$\n",
    "\n",
    "<a name=\"17\"></a>$\\mathbf{P}_{k|k} = (\\mathbf{P}_{k|k-1}^{-1} - \\theta \\cdot \\mathbf{\\tilde{S}}_{k} + \\mathbf{H}_{k}^{\\top} \\mathbf{R}_{k}^{-1} \\mathbf{H}_{k} )^{-1} \\quad (17),$\n",
    "\n",
    "<a name=\"18\"></a>$\\mathbf{K}_{k} = \\mathbf{P}_{k|k}{{\\mathbf{H}_{k}^\\top}}\\mathbf{R}_{k}^{-1} \\quad (18),$\n",
    "\n",
    "<a name=\"19\"></a>$\\mathbf{x}_{k|k} = \\mathbf{x}_{k|k-1} + \\mathbf{K}_{k}\\mathbf{y}_{k} \\quad (19),$\n",
    "\n",
    "## Where:\n",
    "$ \\mathbf{\\bar{S}}_{k} \\gt 0$ is user defined matrix, \n",
    "$ \\mathbf{L}_{k} $ is full rank user defined state weigthing matrix,\n",
    "$ \\theta $ is user defined performance bounary value.\n",
    "\n",
    "# Filtering algorithms comparizon\n",
    "If we compare equations [(10)](#10) and [(17)](#17) then we cen see that the least equation can be computed in two steps:\n",
    "\n",
    "<a name=\"20\"></a>$\\mathbf{P}_{b} = (\\mathbf{P}_{b-1}^{-1} - \\theta \\cdot \\mathbf{\\tilde{S}}_{b})^{-1} = \\mathbf{P}_{b-1} + \\Delta \\mathbf{Q}_{b} \\quad (20),$\n",
    "\n",
    "<a name=\"21\"></a>$\\mathbf{P}_{d} = (\\mathbf{P}_{d-1}^{-1} + \\mathbf{H}_{d}^{\\top} \\mathbf{R}_{d}^{-1} \\mathbf{H}_{d} )^{-1} \\quad (21),$\n",
    "\n",
    "The order of these steps may vary, but the result should be ste same. \n",
    "\n",
    "The step [(21)](#21) is exactly the same as [(10)](#10) which is used in the Kalman filter state covariance update.\n",
    "\n",
    "The step [(20)](#20) can be viewed as an additional process noise.\n",
    "\n",
    "# Adaptive correction derivation\n",
    "## Divergenсe criteria\n",
    "Kalman filter divergence is detected when the folowing critera is met:\n",
    "\n",
    "<a name=\"21\"></a> $\\mathbf{y}_{b}^{\\top} \\mathbf{S}_{b}^\\mathsf{-1} \\mathbf{y}_{b} \\gt {\\beta}_{n} \\quad (21),$\n",
    "\n",
    "where ${\\beta}_{n}$ is threshold ${\\chi}_{\\alpha,n}^{2}$ value.\n",
    "\n",
    "## Correction: Initial derivation\n",
    "\n",
    "After adaptive correction step case we get:\n",
    "\n",
    "<a name=\"22\"></a> $\\mathbf{y}_{b}^\\top \\mathbf{S}_{corr}^\\mathsf{-1} \\mathbf{y}_{b} = {\\beta}_{n} \\quad (22),$\n",
    "\n",
    "By multimlication of the equation [(22)](#22) by $\\mathbf{y}_{b}$ on the left and by $\\mathbf{y}_{b} ^ {\\top}$ on the rigth sides we get:\n",
    "\n",
    "<a name=\"23\"></a> $\\mathbf{y}_{b} \\mathbf{y}_{b}^{\\top} \\mathbf{S}_{corr}^\\mathsf{-1} \\mathbf{y}_{b} \\mathbf{y}_{b}^{\\top} = {\\beta}_{n} \\cdot \\mathbf{y}_{b} \\mathbf{y}_{b}^{\\top} \\quad (23),$\n",
    "\n",
    "By compating left and igth sides of the equation [(23)](#23) we get:\n",
    "\n",
    "$\\mathbf{y}_{b} {y}_{b}^{\\top} \\mathbf{S}_{corr}^{\\mathsf{-1}} = {\\beta}_{n} \\cdot \\mathbf{I} ,$\n",
    "\n",
    "or\n",
    "\n",
    "$\\mathbf{y}_{b} \\mathbf{y}_{b}^{\\top} = {\\beta}_{n} \\cdot \\mathbf{S}_{corr} ,$\n",
    "\n",
    "or\n",
    "\n",
    "<a name=\"24\"></a> $\\mathbf{S}_{corr} = \\cfrac {\\mathbf{y}_{b} \\mathbf{y}_{b}^{\\top}} {{\\beta}_{n}} \\quad (24),$\n",
    "\n",
    "## Correction: No limits approach\n",
    "\n",
    "By substitution of [(20)](#20) rigth side to [(16)](#16) we get:\n",
    "\n",
    "<a name=\"25\"></a> $\\mathbf{S}_{corr} = {S}_{b} + {\\mathbf{H}_{b}} {\\Delta \\mathbf{Q}_{b}} {\\mathbf{H}_{b}^{\\top}} \\quad (25),$\n",
    "\n",
    "and so substitution [(25)](#25) to [(24)](#24) gives us:\n",
    "\n",
    "<a name=\"26\"></a> ${S}_{b} + {\\mathbf{H}_{b}} {\\Delta \\mathbf{Q}_{b}} {\\mathbf{H}_{b}^{\\top}} = \\cfrac {\\mathbf{y}_{b} \\mathbf{y}_{b}^{\\top}} {{\\beta}_{n}} \\quad (26),$\n",
    "\n",
    "or \n",
    "\n",
    "<a name=\"27\"></a> $ {A}_{b} = {\\mathbf{H}_{b}} {\\Delta \\mathbf{Q}_{b}} {\\mathbf{H}_{b}^{\\top}} = \\cfrac {\\mathbf{y}_{b} \\mathbf{y}_{b}^{\\top}} {{\\beta}_{n}} - {S}_{b} \\quad (27),$\n",
    "\n",
    "on the other hand [(20)](#20) gives us:\n",
    "\n",
    "$ \\mathbf{P}_{b} = (\\mathbf{P}_{b-1}^{-1} - \\theta \\cdot \\mathbf{\\tilde{S}}_{b})^{-1} = \\mathbf{P}_{b-1} + \\Delta \\mathbf{Q}_{b} $\n",
    "\n",
    "or \n",
    "\n",
    "$ \\mathbf{P}_{b} = (\\mathbf{P}_{b-1}^{-1} - \\theta \\cdot {\\mathbf{L}_{b}^{\\top}} \\mathbf{\\bar{S}}_{b} {\\mathbf{L}_{b}})^{-1} = (\\mathbf{P}_{b-1}^{-1} - {\\mathbf{L}_{b}^{\\top}} \\mathbf{M}_{b}^{-1} {\\mathbf{L}_{b}})^{-1} \\quad ,$ \n",
    "where $\\mathbf{M}_{b}^{-1} =  \\theta \\cdot \\mathbf{\\bar{S}}_{b} $\n",
    "\n",
    "or \n",
    "\n",
    "$ \\mathbf{P}_{b} = \\mathbf{P}_{b-1} + \\mathbf{P}_{b-1}  {\\mathbf{L}_{b}^{\\top}} \\left(\\mathbf{M}_{b} - {\\mathbf{L}_{b}} {\\mathbf{P}_{b-1}} {\\mathbf{L}_{b}^{\\top}} \\right)^{-1} {\\mathbf{L}_{b}} \\mathbf{P}_{b-1} $\n",
    "\n",
    "which means that:\n",
    "\n",
    "<a name=\"28\"></a> $ {\\Delta \\mathbf{Q}_{b}} = \\mathbf{P}_{b-1}  {\\mathbf{L}_{b}^{\\top}} \\left(\\mathbf{M}_{b} - {\\mathbf{L}_{b}} {\\mathbf{P}_{b-1}} {\\mathbf{L}_{b}^{\\top}} \\right)^{-1} {\\mathbf{L}_{b}} \\mathbf{P}_{b-1} \\quad (28),$\n",
    "\n",
    "from [(27)](#27) we get:\n",
    "\n",
    "$ \\mathbf{A}_{b} = {\\mathbf{H}_{b}} {\\Delta \\mathbf{Q}_{b}} {\\mathbf{H}_{b}^{\\top}} = {\\mathbf{H}_{b}} {\\mathbf{P}_{b-1}  {\\mathbf{L}_{b}^{\\top}} \\left(\\mathbf{M}_{b} - {\\mathbf{L}_{b}} {\\mathbf{P}_{b-1}} {\\mathbf{L}_{b}^{\\top}} \\right)^{-1} {\\mathbf{L}_{b}} \\mathbf{P}_{b-1}} {\\mathbf{H}_{b}^{\\top}} = \\mathbf{C}_{b} {\\left(\\mathbf{M}_{b} - {\\mathbf{L}_{b}} {\\mathbf{P}_{b-1}} {\\mathbf{L}_{b}^{\\top}} \\right)^{-1}} \\mathbf{C}_{b}^{\\top} $\n",
    "\n",
    "or \n",
    "\n",
    "$ \\mathbf{A}_{b} = \\mathbf{C}_{b} {\\left(\\mathbf{M}_{b} - {\\mathbf{L}_{b}} {\\mathbf{P}_{b-1}} {\\mathbf{L}_{b}^{\\top}} \\right)^{-1}} \\mathbf{C}_{b}^{\\top} $\n",
    "\n",
    "or \n",
    "\n",
    "$ \\mathbf{C}_{b}^{+} \\mathbf{A}_{b} = {\\left(\\mathbf{M}_{b} - {\\mathbf{L}_{b}} {\\mathbf{P}_{b-1}} {\\mathbf{L}_{b}^{\\top}} \\right)^{-1}} \\mathbf{C}_{b}^{\\top} $\n",
    "\n",
    "or\n",
    "\n",
    "$ {\\left(\\mathbf{M}_{b} - {\\mathbf{L}_{b}} {\\mathbf{P}_{b-1}} {\\mathbf{L}_{b}^{\\top}} \\right)} \\mathbf{C}_{b}^{+} = \\mathbf{C}_{b}^{\\top} \\mathbf{A}_{b}^{-1}$\n",
    "\n",
    "or\n",
    "\n",
    "$ \\mathbf{M}_{b} - {\\mathbf{L}_{b}} {\\mathbf{P}_{b-1}} {\\mathbf{L}_{b}^{\\top}} = \\mathbf{C}_{b}^{\\top} \\mathbf{A}_{b}^{-1} \\mathbf{C}_{b}$\n",
    "\n",
    "or\n",
    "\n",
    "<a name=\"29\"></a> $ \\mathbf{M}_{b} = \\mathbf{C}_{b}^{\\top} \\mathbf{A}_{b}^{-1} \\mathbf{C}_{b} + {\\mathbf{L}_{b}} {\\mathbf{P}_{b-1}} {\\mathbf{L}_{b}^{\\top}} \\quad (29),$\n",
    "\n",
    "\n",
    "where:\n",
    "\n",
    "<a name=\"30\"></a> $ \\mathbf{C}_{b} = {\\mathbf{L}_{b}} \\mathbf{P}_{b-1} {\\mathbf{H}_{b}^{\\top}} \\quad (30),$\n",
    "\n",
    "so for $\\Delta \\mathbf{Q}_{b}$ we have:\n",
    "\n",
    "$ {\\Delta \\mathbf{Q}_{b}} = \\mathbf{P}_{b-1}  {\\mathbf{L}_{b}^{\\top}} \\left(\\mathbf{C}_{b}^{\\top} \\mathbf{A}_{b}^{-1} \\mathbf{C}_{b} + {\\mathbf{L}_{b}} {\\mathbf{P}_{b-1}} {\\mathbf{L}_{b}^{\\top}} - {\\mathbf{L}_{b}} {\\mathbf{P}_{b-1}} {\\mathbf{L}_{b}^{\\top}} \\right)^{-1} {\\mathbf{L}_{b}} \\mathbf{P}_{b-1}  = \\mathbf{P}_{b-1}  {\\mathbf{L}_{b}^{\\top}} \\left(\\mathbf{C}_{b}^{\\top} \\mathbf{A}_{b}^{-1} \\mathbf{C}_{b} \\right)^{-1} {\\mathbf{L}_{b}} \\mathbf{P}_{b-1} $\n",
    "\n",
    "or \n",
    "\n",
    "<a name=\"31\"></a> $ {\\Delta \\mathbf{Q}_{b}} = \\mathbf{P}_{b-1} \\mathbf{L}_{b}^{\\top} \\mathbf{C}_{b}^{+} \\mathbf{A}_{b} \\mathbf{C}_{b}^{+ \\top} \\mathbf{L}_{b} \\mathbf{P}_{b-1}  \\quad (31),$\n",
    "\n",
    "\n",
    "# References\n",
    "\n",
    "<a name=\"banavar\"></a> **[Banavar1992]** R. Banavar, “A game theoretic approach to linear dynamic estimation”, Doctoral Dissertation,\n",
    "University of Texas at Austin, May 1992.\n"
   ]
  },
  {
   "cell_type": "markdown",
   "metadata": {},
   "source": [
    "$\\left(A + UCV\\right)^{-1} = A^{-1} - A^{-1}U \\left(C^{-1}+VA^{-1}U \\right)^{-1}VA^{-1}$\n",
    "\n",
    "\n",
    "$\\left(A + UBV\\right)^{-1} = A^{-1} - A^{-1}UB\\left(B+BVA^{-1}UB\\right)^{-1}BVA^{-1}$\n",
    "\n",
    "\n",
    "$ {A}_{b} = {\\mathbf{H}_{k}} {\\Delta \\mathbf{Q}_{b}} {\\mathbf{H}_{k}^{\\top}} = {\\mathbf{H}_{k}} {\\mathbf{P}_{b-1}  {\\mathbf{L}_{b}^{\\top}} \\left(\\mathbf{M}_{b} - {\\mathbf{L}_{b}} {\\mathbf{P}_{b-1}} {\\mathbf{L}_{b}^{\\top}} \\right)^{-1} {\\mathbf{L}_{b}} \\mathbf{P}_{b-1}} {\\mathbf{H}_{k}^{\\top}}$\n"
   ]
  },
  {
   "cell_type": "code",
   "execution_count": null,
   "metadata": {},
   "outputs": [],
   "source": [
    "="
   ]
  }
 ],
 "metadata": {
  "kernelspec": {
   "display_name": "Python 3",
   "language": "python",
   "name": "python3"
  },
  "language_info": {
   "codemirror_mode": {
    "name": "ipython",
    "version": 3
   },
   "file_extension": ".py",
   "mimetype": "text/x-python",
   "name": "python",
   "nbconvert_exporter": "python",
   "pygments_lexer": "ipython3",
   "version": "3.6.12"
  }
 },
 "nbformat": 4,
 "nbformat_minor": 4
}
